More.

theories/common/treemap.v
@@ -14,16 +14,44 @@ Section treemap_rooted.
 
   Implicit Types node root src dst : N.
   Implicit Types edge : E.
-  Implicit Types δ : E * N.
+  Implicit Types edges : list E.
+  Implicit Types ϵ : N * E.
   Implicit Types tree : treemap N E.
 
-  Parameter treemap_rooted : treemap N E → N → Prop.
+  Inductive treemap_path tree dst : N → list E → Prop :=
+    | treemap_path_nil :
+        treemap_path tree dst dst []
+    | treemap_path_cons {node1} ϵ node2 edge edges :
+        tree !! node1 = Some ϵ →
+        ϵ.1 = node2 →
+        ϵ.2 = edge →
+        treemap_path tree dst node2 edges →
+        treemap_path tree dst node1 (edge :: edges).
+  #[local] Hint Constructors treemap_path : core.
 
-  Axiom treemap_rooted_empty : ∀ root,
+  Definition treemap_rooted tree root :=
+    ∀ node,
+    is_Some (tree !! node) →
+      ∃ edges,
+      treemap_path tree root node edges.
+
+  Lemma treemap_rooted_empty root :
     treemap_rooted ∅ root.
+  Proof.
+    intros node []%(lookup_empty_is_Some (A := N * E)).
+  Qed.
 
   Axiom treemap_rooted_lift : ∀ {tree root} root_edge root',
     treemap_rooted tree root →
     tree !! root' = None →
     treemap_rooted (<[root := (root', root_edge)]> tree) root'.
+
+  Lemma treemap_rooted_path {tree root} node :
+    treemap_rooted tree root →
+    is_Some (tree !! node) →
+      ∃ edges,
+      treemap_path tree root node edges.
+  Proof.
+    auto.
+  Qed.
 End treemap_rooted.
